src/reflection/FStar.Reflection.Data.fs
@@ -50,14 +50,11 @@ type comp_view =
     | C_Lemma of term * term
     | C_Unknown
 
-// See ulib/FStar.Reflection.Syntax.fst for explanations of these two
-type ctor =
-    | Ctor of  name * typ
 type sigelt_view =
-    | Sg_Inductive of name * list<binder> * typ * list<ctor>
     | Sg_Let of fv * typ * term
+    | Sg_Inductive of name * list<binder> * typ * list<name> // name, params, type, constructors
+    | Sg_Constructor of name * typ
     | Unk
-
 
 (* Contains all lids and terms needed for embedding/unembedding *)
 
@@ -88,15 +85,17 @@ let fstar_refl_pack        = fvar fstar_refl_pack_lid (Delta_defined_at_level 1)
 let fstar_refl_pack_fv_lid = fstar_refl_basic_lid "pack_fv"
 let fstar_refl_pack_fv     = fvar fstar_refl_pack_fv_lid (Delta_defined_at_level 1) None
 
-(* types *)
-let fstar_refl_aqualv    = mk_refl_data_lid_as_term "aqualv"
+(* assumed types *)
 let fstar_refl_env       = mk_refl_types_lid_as_term "env"
 let fstar_refl_fv        = mk_refl_types_lid_as_term "fv"
 let fstar_refl_comp      = mk_refl_types_lid_as_term "comp"
-let fstar_refl_comp_view = mk_refl_data_lid_as_term "comp_view"
 let fstar_refl_binder    = mk_refl_types_lid_as_term "binder"
+let fstar_refl_sigelt    = mk_refl_types_lid_as_term "sigelt"
+
+(* auxiliary types *)
+let fstar_refl_aqualv    = mk_refl_data_lid_as_term "aqualv"
+let fstar_refl_comp_view = mk_refl_data_lid_as_term "comp_view"
 let fstar_refl_term_view = mk_refl_data_lid_as_term "term_view"
-let fstar_refl_ctor      = mk_refl_data_lid_as_term "ctor"
 let fstar_refl_pattern   = mk_refl_data_lid_as_term "pattern"
 let fstar_refl_branch    = mk_refl_data_lid_as_term "branch"
 
@@ -137,10 +136,10 @@ let ref_C_Lemma   = fstar_refl_data_const "C_Lemma"
 let ref_C_Unknown = fstar_refl_data_const "C_Unknown"
 
 (* inductives & sigelts *)
-let ref_Sg_Inductive = fstar_refl_data_const "Sg_Inductive"
-let ref_Sg_Let       = fstar_refl_data_const "Sg_Let"
-let ref_Unk          = fstar_refl_data_const "Unk"
-let ref_Ctor         = fstar_refl_data_const "Ctor"
+let ref_Sg_Let         = fstar_refl_data_const "Sg_Let"
+let ref_Sg_Inductive   = fstar_refl_data_const "Sg_Inductive"
+let ref_Sg_Constructor = fstar_refl_data_const "Sg_Constructor"
+let ref_Unk            = fstar_refl_data_const "Unk"
 
 (* Should not be here *)
 let ord_Lt_lid = Ident.lid_of_path (["FStar"; "Order"; "Lt"]) Range.dummyRange
