ulib/FStar.Reflection.Types.fsti
@@ -5,6 +5,7 @@ assume new type term
 assume new type env
 assume new type fv
 assume new type comp
+assume new type sigelt
 
 type name : eqtype = list string
 type typ     = term
